powerpc/Asmgenproof.v
@@ -1322,7 +1322,7 @@ Proof.
 Qed.
 
 Theorem transf_program_correct:
-  forall (beh: program_behavior),
+  forall (beh: program_behavior), not_wrong beh ->
   Machconcr.exec_program prog beh -> Asm.exec_program tprog beh.
 Proof.
   unfold Machconcr.exec_program, Asm.exec_program; intros.
